basic placeholder setup for program equiv

EffectSSA/Rewrites/Basic.lean
@@ -40,20 +40,23 @@ def Rewrite.WellFormed (Γ : Context τ) (r : Rewrite τ) : Prop :=
 -/
 variable {τ} [MemoryModel τ]
 
--- TODO: ProgramFragment.append
--- TODO: ProgramFragment.execClosed
-
 /--
-A rewrite is correct, if the source and target fragments compute the same values
-for the return variables (given the same environment).
+A rewrite is correct, if the source and target fragments are equivalent.
 -/
 def Rewrite.Correct (r : Rewrite τ) : Prop :=
-  ∃ (Δ : Context τ) (ts : _),
-    r.src.WellTyped Δ ts
-    ∧ r.tgt.WellTyped Δ ts
-    ∧ ∀ (C : Program τ), C.WellTyped ∅ Δ.toList →
-          (C ++ r.src).execClosed? = (C ++ r.tgt).execClosed?
-  -- FIXME: this is actually too granular, as it looks for strict equality of
-  --        of traces, whereas we want to consider something a bit looser, e.g.
-  --        to disregard the specific order of load events.
-  -- ∀ {env} {Γ}, env.WellTyped Γ → r.src.exec env = r.tgt.exec env
+  r.src ≈ r.tgt
+
+
+/-!
+## Lemmas
+--------------------------------------------------------------------------------
+-/
+
+/--
+Only wellformed rewrites can be correct
+-/
+theorem Rewrite.wellFormed_of_correct (h : Correct r) : ∃ Γ, WellFormed Γ r := by
+  -- TODO: this does not actually hold under the current placeholder definition
+  -- of program equivalence, but it likely should hold under the actual eventual
+  -- definition
+  sorry
