EffectSSA/Semantics/Equiv.lean
@@ -1,1 +1,2 @@
 import EffectSSA.Semantics.Equiv.ClosingContext
+import EffectSSA.Semantics.Equiv.Equiv
