EffectSSA/Semantics/Equiv/Equiv.lean
@@ -1,0 +1,34 @@
+import EffectSSA.Syntax
+import EffectSSA.Semantics.Equiv.ClosingContext
+import EffectSSA.Semantics.Program
+import EffectSSA.Semantics.Lemmas
+
+/-!
+# Program Equivalence
+-/
+namespace EffectSSA
+namespace Program
+
+@[grind =]
+def Equiv (p : Program τ) (q : Program τ) : Prop :=
+  -- TODO: this is just a placeholder, the actual definition should
+  -- refer to contexts
+  p = q
+
+instance : Setoid (Program τ) where
+  r := Equiv
+  iseqv := {
+    refl := by grind
+    symm := by grind
+    trans := by grind
+  }
+
+/-!
+## Lemmas
+--------------------------------------------------------------------------------
+-/
+section Lemmas
+variable {p q : Program τ}
+
+/-- `_ ≈ _` is the preferred spelling -/
+theorem equiv_iff : p.Equiv q ↔ p ≈ q := by rfl
